<?xml version="1.0"?>
<rdf:RDF
    xmlns:rdf="http://www.w3.org/1999/02/22-rdf-syntax-ns#"
    xmlns:rdfs="http://www.w3.org/2000/01/rdf-schema#"
    xml:base="http://vapour.sourceforge.net/vocab.rdf"    
    >

  <rdf:Property rdf:about="#previousSubject">
    <rdfs:label xml:lang="en">The previous HTTP dialogue</rdfs:label>
    <rdfs:comment xml:lang="en">Some dereferences require more than
    one HTTP request/response dialogue, because the first response
    contains an HTTP 303 REDIRECT code. This property connects a
    dialogue fragment with the inmediate previous one.</rdfs:comment>
    <rdfs:domain rdf:resource="http://www.w3.org/WAI/ER/EARL/nmg-strawman#TestSubject"/>
    <rdfs:range rdf:resource="http://www.w3.org/WAI/ER/EARL/nmg-strawman#TestSubject"/>
  </rdf:Property>

  <rdf:Property rdf:about="#previousRequestCount">
    <rdfs:label xml:lang="en">Number of previous request</rdfs:label>
    <rdfs:comment xml:lang="en">The number of HTTP requests previous to this one (i.e.: hop-count)</rdfs:comment>
    <rdfs:domain rdf:resource="http://www.w3.org/WAI/ER/EARL/nmg-strawman#TestSubject"/>
    <!--rdfs:range rdf:resource=""/-->  <!-- FIXME: xs:integer -->
  </rdf:Property>

  <rdf:Property rdf:about="#propertyUnderTest">
    <rdfs:label xml:lang="en">
      Property under test
    </rdfs:label>
    <rdfs:comment xml:lang="en">
      The property of the HTTP which value is checked in this test.
    </rdfs:comment>
    <rdfs:domain rdf:resource="http://www.w3.org/WAI/ER/EARL/nmg-strawman#TestCase"/>
  </rdf:Property>

  <rdf:Property rdf:about="#order">
    <rdfs:label xml:lang="en">
      Order (priority, position) of the test requirement
    </rdfs:label>
    <rdfs:comment xml:lang="en">
      This property is used for presentational purposes, just to define an
      convenient order for the test requirements
    </rdfs:comment>
    <rdfs:domain rdf:resource="http://www.w3.org/WAI/ER/EARL/nmg-strawman#TestRequirement"/>
  </rdf:Property>

  <rdf:Property rdf:about="#httpRange14ConclusionOn">
    <rdfs:label xml:lang="en">
      Derives a conclusion on the type of
    </rdfs:label>
    <rdfs:comment xml:lang="en">
      This property relates a TestSubject with a web resource which type
      can be inferred as per httpRange-14 TAG finding
    </rdfs:comment>
    <rdfs:domain rdf:resource="http://www.w3.org/WAI/ER/EARL/nmg-strawman#TestSubject"/>
  </rdf:Property>

  <rdfs:Class rdf:about="#AnyResource">
    <rdfs:label xml:lang="en">
      Any kind of web resource
    </rdfs:label>
  </rdfs:Class>

  <rdfs:Class rdf:about="#InformationResource">
    <rdfs:subClassOf rdf:resource="#AnyResource"/>
    <rdfs:label xml:lang="en">
      Information resource
    </rdfs:label>
  </rdfs:Class>

</rdf:RDF>
